cfrontend/BeePL_ebpf_proofs.v
@@ -7,18 +7,188 @@ Require Import BeePL_sem BeePL_typesystem BeePL_safety BeePL_typesystem_proofs.
 
 From mathcomp Require Import all_ssreflect.
 
+(****** No divergence effect ********)
+Lemma no_divergence_type_system :
+(forall cenv Gamma Sigma es efs ts, 
+ type_exprs cenv Gamma Sigma es efs ts ->
+ no_divergence efs) /\
+(forall cenv Gamma Sigma e ef t, 
+ type_expr cenv Gamma Sigma e ef t ->
+ no_divergence ef).
+Proof.
+suff : (forall cenv Gamma Sigma es efs ts, 
+ type_exprs cenv Gamma Sigma es efs ts ->
+ no_divergence efs) /\
+(forall cenv Gamma Sigma e ef t, 
+ type_expr cenv Gamma Sigma e ef t ->
+ no_divergence ef).
++ move=> [] h1 h2. by split=> //=.
+apply type_exprs_type_expr_ind_mut=> //=.
+(* app *)
++ move=> cenv Gamma Sigma e te es rt efs ts ef efs' hte hd hteq hts hds. apply no_divergence_concat.
+  + by apply hd. apply no_divergence_concat. 
+  + admit.
+  (* here function signature has the effect of the body also, how to ensure that there is no divergence in the effect of body *)
+  by apply hds.
+(* ref *)
++ move=> cenv Gamma Sigma e ef h bt a he hd. by apply no_divergence_concat.
+(* deref *)
++ move=> cenv Gamma Sigma e ef h bt a he hd. by apply no_divergence_concat.
+(* massgn *)
++ move=> cenv Gamma Sigma e e' h pt ef ef' hte hd1 hte' hd2. apply no_divergence_concat.
+  + by apply hd1.
+  by apply no_divergence_concat.
++ move=> cenv Gamma Sigma e ef1 ef2 t e' hteq hte1 hd1 hte2 hd2. by apply no_divergence_concat.
++ move=> cenv Gamma Sigma e ef1 ef2 t e' hteq hte1 hd1 hte2 hd2. by apply no_divergence_concat.
++ move=> cenv Gamma Sigma e ef1 ef2 t e' hteq hte1 hd1 hte2 hd2. by apply no_divergence_concat.
++ move=> cenv Gamma Sigma e ef1 ef2 t e' hteq hte1 hd1 hte2 hd2. by apply no_divergence_concat.
++ move=> cenv Gamma Sigma e ef1 ef2 t e' hteq hte1 hd1 hte2 hd2. by apply no_divergence_concat.
++ move=> cenv Gamma Sigma e ef1 ef2 t e' hteq hte1 hd1 hte2 hd2. by apply no_divergence_concat.
++ move=> cenv Gamma Sigma e ef1 ef2 t e' hteq hte1 hd1 hte2 hd2. by apply no_divergence_concat.
++ move=> cenv Gamma Sigma e ef1 ef2 t e' hteq hte1 hd1 hte2 hd2. by apply no_divergence_concat.
++ move=> cenv Gamma Sigma e ef1 ef2 t e' hteq hte1 hd1 hte2 hd2. by apply no_divergence_concat.
++ move=> cenv Gamma Sigma e ef1 ef2 t e' hteq hte1 hd1 hte2 hd2. by apply no_divergence_concat.
++ move=> cenv Gamma Sigma e ef1 ef2 t e' hteq hte1 hd1 hte2 hd2. by apply no_divergence_concat.
++ move=> cenv Gamma Sigma e ef1 ef2 t e' hteq hte1 hd1 hte2 hd2. by apply no_divergence_concat.
++ move=> cenv Gamma Sigma e ef1 ef2 t e' hteq hte1 hd1 hte2 hd2. by apply no_divergence_concat.
++ move=> cenv Gamma Sigma e ef1 ef2 t e' hteq hte1 hd1 hte2 hd2. by apply no_divergence_concat.
++ move=> cenv Gamma Sigma e ef1 ef2 t e' hteq hte1 hd1 hte2 hd2. by apply no_divergence_concat.
++ move=> cenv Gamma Sigma e ef1 ef2 t e' hteq hte1 hd1 hte2 hd2. by apply no_divergence_concat.
++ move=> cenv Gamma Sigma e ef1 ef2 t e' hteq hte1 hd1 hte2 hd2. by apply no_divergence_concat.
++ move=> cenv Gamma Sigma e1 e2 e3 t ef1 ef2 hte1 hd1 hte2 hd2 hte3 hd3. by apply no_divergence_concat.
++ move=> cenv Gamma Sigma e1 e2 d e ef1 t1 ef2 t2 fv1 fv2 fv ef t hte1 hd1 hte2 hd2 hte hd heq hil hfv1 hfv2
+         hfv hdis1 hdis2. apply no_divergence_concat. + by apply hd1. + by apply no_divergence_concat.
++ move=> cenv Gamma Sigma e ef te ps es efs ts fvs hg hte hd htes hds ho ha. by apply no_divergence_concat.
+move=> cenv Gamma Sigma e es ef efs t ts hte hd htes hds. by apply no_divergence_concat.
+Admitted.
+
+ 
+(*Lemma no_divergence_sem :
+(forall cenv Gamma Sigma es efs ts bge p vm m m' vm' es', 
+ type_exprs cenv Gamma Sigma es efs ts ->
+ ssem_exprs bge p vm m es m' vm' es' ->
+ no_divergence efs) /\
+(forall cenv Gamma Sigma e ef t bge p vm m m' vm' e', 
+ type_expr cenv Gamma Sigma e ef t ->
+ ssem_expr bge p vm m e m' vm' e' ->
+ no_divergence ef).
+Proof.
+suff : (forall cenv Gamma Sigma es efs ts, type_exprs cenv Gamma Sigma es efs ts ->
+           forall  bge p vm m m' vm' es', ssem_exprs bge p vm m es m' vm' es' ->
+                                          no_divergence efs) /\
+       (forall cenv Gamma Sigma e ef t, type_expr cenv Gamma Sigma e ef t ->
+           forall bge p vm m m' vm' e', ssem_expr bge p vm m e m' vm' e' ->
+                                        no_divergence ef).
++ admit.
+apply type_exprs_type_expr_ind_mut=> //=.
+(* app *)
++ admit.
+(* ref *)
++ move=> cenv Gamma Sigma e ef h bt a hte hin bge p vm m m' vm' e' he.
+  inversion he; subst.
+  + move: (hin bge p vm m m' vm' e'0 H9)=> hd. by apply no_divergence_concat.
+  have hv : ssem_expr bge p vm m (Val v (construct_type_btype bt)) m vm (Val v (construct_type_btype bt)).
+  + apply ssem_value. 
+    by have := typed_well_formed_value cenv Gamma Sigma v (construct_type_btype bt) ef hte.
+    move: (hin bge p vm m m vm  (Val v (construct_type_btype bt)) hv)=> hd.
+  by apply no_divergence_concat.
+(* deref *)
++ admit.
+(* massgn *)
++ admit.
+(* onotbool *)
++ admit.
+(* onotint *)
++ admit.
+(* oneg *)
++ admit.
+(* oadd *)
++ admit.
+(* osub *)
++ admit.
+(* omul *)
++ admit.
+(* odiv *)
++ admit.
+(* omod *)
++ admit.
+(* oand *)
++ admit.
+(* oor *)
++ admit.
+(* oxor *)
++ admit.
+(* oshl *)
++ admit.
+(* oshr *)
++ admit.
+(* oeq *)
++ admit.
+(* one *)
++ admit.
+(* olt *)
++ admit.
+(* ogt *)
++ admit.
+(* ole *)
++ admit.
+(* oge *)
++ admit.
+(* bind *)
++ move=> cenv Gamma Sigma x t e e' t' ef ef' hte hin hte' hin' bge p vm m m' vm' e'' he.
+  inversion he; subst.
+  (* step *)
+  + move: (hin bge p vm m m' vm' e1' H10)=> hd1. 
+    have [h1 h2] := no_divergence_type_system.
+    move: (h2 cenv (extend_context Gamma x t) Sigma e' ef' (typeof_expr e') hte')=> hd2.
+    by apply no_divergence_concat.
+  (* value *)
+   have [h1 h2] := no_divergence_type_system.
+   move: (h2 cenv (extend_context Gamma x t) Sigma e' ef' (typeof_expr e') hte')=> hd2.
+    
+Admitted. *) 
+
 (***** Termination *****)
 (* A well typed program where the effects contain no divergence effect is always terminating *)
 Lemma guaranteed_termination : 
-(forall Gamma Sigma es efs ts bge vm m n m' vm' es', 
- type_exprs Gamma Sigma es efs ts ->
- no_divergence efs ->
- ssem_closures bge vm m es n m' vm' es' ->
- exists m, (n <= m)%nat) /\
-(forall Gamma Sigma e ef t bge vm m n m' vm' e', 
- type_expr Gamma Sigma e ef t ->
- no_divergence ef ->
- ssem_closure bge vm m e n m' vm' e' ->
- exists m, (n <= m)%nat).
+(forall cenv Gamma Sigma es efs ts bge p vm m, 
+ type_exprs cenv Gamma Sigma es efs ts ->
+ store_well_typed Gamma Sigma bge vm m ->
+ exists n m' vm' vs, ssem_closures bge p vm m es n m' vm' vs /\ is_values vs /\ no_divergence efs) /\
+(forall cenv Gamma Sigma e ef t bge p vm m, 
+ type_expr cenv Gamma Sigma e ef t ->
+ store_well_typed Gamma Sigma bge vm m ->
+ exists n m' vm' v, ssem_closure bge p vm m e n m' vm' v /\ is_value v /\ no_divergence ef).
 Proof.
+suff : (forall cenv Gamma Sigma es efs ts, 
+           type_exprs cenv Gamma Sigma es efs ts ->
+           forall bge p vm m, store_well_typed Gamma Sigma bge vm m -> exists n m' vm' vs, 
+                                                  ssem_closures bge p vm m es n m' vm' vs /\
+                                                  is_values vs /\ no_divergence efs) /\
+       (forall cenv Gamma Sigma e ef t, 
+           type_expr cenv Gamma Sigma e ef t ->
+           forall bge p vm m, store_well_typed Gamma Sigma bge vm m -> exists n m' vm' v, 
+                                                 ssem_closure bge p vm m e n m' vm' v /\
+                                                  is_value v /\ no_divergence ef).
++ admit.
+apply type_exprs_type_expr_ind_mut=> //=.
+(* Val unit *)
++ move=> cenv Gamma Sigma bge p vm m. exists 0%N. exists m.
+  exists vm. exists (Val BeePL_values.Vunit BeePL_notations.tunit). split=> //=.
+  by apply ssem_val.
+(* Val bool *)
++ move=> cenv Gamma Sigma b bge p vm m. exists 0%N. exists m.
+  exists vm. exists (Val (BeePL_values.Vbool b) (Vtype Tbool)). split=> //=.
+  by apply ssem_val.
+(* Val int *)
++ admit. (* easy *)
+(* Val long *) 
++ admit. (* easy *)
+(* Val loc *)
++ admit. (* easy *)
+(* Var *)
++ move=> cenv Gamma Sigma x t hx bge p vm m hw. inversion hw.
+  + move: (H x t hx)=> [] l' [] t' [] v [] ofs [] h1 [] h2 [] h3 [] hd [] hf h; subst.
+    exists 1%N. exists m. exists vm. exists (Val v t'); split=> //=. apply ssem_one.
+    by apply ssem_lvar with l' ofs. 
 Admitted.
